---
title: Intro Prob Lecture Notes
author:
    - William Sun
date:
    - April 28, 2017
geometry: margin=3cm
header-includes:
    - \usepackage{setspace}
    - \doublespacing
---
- Some stuff I missed...
- Two important properties:
#) If $X, Y$ are independent... etc
#) If $X, Y$ have the same MGF, then $X,Y$ have to have the same probability distribution. 
	- When they exist, they uniquely identify the distribution of a random variable. That is, two different distributions cannot lead to the same MGF.
- Ex: $X \sim$ Poisson($\lambda$). Find the MGF if it exists
\begin{align*}
	M_X(t) &= E(e^{tX}) \\
	&= \sum\limits_{x = 0}^{\infty} e^{tx} \frac{e^{-\lambda} \lambda^x}{x!} \\
	&= e^{-\lambda} \sum\limits_{x = 0}^{\infty} \frac{(\lambda e^t)^2}{x!} \\
	&= e^{-\lambda} e^{\lambda e^t} \\
	&= e^{\lambda (e^t - 1)}
\end{align*}
- Homework (expectation): Compute MGF of Gamma($\alpha, beta$) to be $(1 - \beta t)^{- \alpha}$
- Ex: $Z \sim$ Normal(0, 1)
\begin{align*}
	E(e^{tZ}) &= \int\limits_{-\infty}^{\infty} e^{tz} \frac{e^{- \frac{z^2}{2}}}{\sqrt{2\pi}} dz \\
	&= \int\limits_{-\infty}^{\infty} \frac{e^{-\frac{1}{2} (z^2 - 2tz)}}{\sqrt{2 \pi}} dz \\
	&= \int\limits_{-\infty}^{\infty} \frac{e^{-\frac{1}{2} (z^2 - 2tz + t^2 - t^2)}}{\sqrt{2 \pi}} dz \\
	&= \int\limits_{-\infty}^{\infty} \frac{e^{-\frac{1}{2} ((z - t)^2 - t^2)}}{\sqrt{2 \pi}} dz \\
	&= e^{\frac{t^2}{2}} \int\limits_{-\infty}^{\infty} \frac{e^{-\frac{(z - t)^2}{2}}}{\sqrt{2 \pi}} dz \\
	&= e^{\frac{t^2}{2}}
\end{align*}
- Recall if $X \sim$ N($\mu, \sigma^2$) then $$X = \mu + \sigma Z$$ So, $$E(e^{tX}) = e^{\mu t + \frac{\sigma^2 t^2}{2}} \text { (Details omitted) }$$
- Ex: Suppose $X_1, X_2 \sim$ independent Poisson($\lambda$)
	- Find the distribution of $X_1 + X_2$ using MGFs
	-
	\begin{align*}
		M_{X_1 + X_2} (t) &= M_{X_1}(t) \cdot M_{X_2}(t) \\
		&= e^{\lambda(e^t - 1)} \cdot e^{\lambda (e^t - 1)} \\
		&= e^{2 \lambda (e^t - 1)}
	\end{align*}
	- Same MGF as MGF of Poisson($2 \lambda$). Therefore the sum IS the Poisson$(2 \lambda)$
- Remark: If $X_1, X_2, \dots, X_n$ are independent then $$M_{\sum\limits_{i = 1}^n X_i} (t) = \prod\limits_{i = 1}^n M_{X_i}(t)$$

# A Central Limit Theorem
- $X_1, X_2, X_3, \dots \sim$ independent Poisson($\lambda$)
- Define $S_n = \sum\limits_{i = 1}^n X_i \sim$ Poisson($n \lambda$)
- Standarize $S_n$ by subtracting the mean and dividing by the variance $Y_n := \frac{S_n - n \lambda}{\sqrt{n \lambda}}$
- Find the MGFA of $Y_n$
-
\begin{align*}
	E(e^{t(\frac{S_n - n \lambda}{\sqrt{n \lambda}})}) &= E(e^{\frac{t}{\sqrt{n \lambda} \cdot S_n}} e^{- \sqrt{n \lambda} t})\\
	&= e^{-\sqrt{n \lambda} t} E(e^{\frac{t}{\sqrt{n \lambda}} \cdot S_n}) \text{ Note: the expectation is MGF } M_{S_n}(\frac{t}{\sqrt{n \lambda}})\\
	&= e^{- \sqrt{n \lambda} t} e^{n \lambda(e^{\frac{t}{\sqrt{n \lambda}}} - 1)} \\
	& \text{ Note: } e^{\frac{t}{\sqrt{n \lambda}}} \approx 1 + \frac{t}{\sqrt{n \lambda}} + \frac{t^2}{2 n \lambda} + \dots \\
	&= e^{\frac{t^2}{2} + \text{ terms with n in denominator }} \rightarrow e^{\frac{t^2}{2}} \\
\end{align*}
- Therefore, it converges to the standard normal distribution