---
title: Intro Prob Lecture Notes
author:
    - William Sun
date:
    - March 27, 2017
geometry: margin=3cm
header-includes:
    - \usepackage{setspace}
    - \doublespacing
---
# Last Time: Gamma PDF
- $X \sim$ Gamma($\alpha, \beta$) where $\alpha > 0, \beta > 0$ has pdf
-
$$f(x) = \frac{x^{\alpha - 1}e^{-\frac{x}{\beta}}}{\beta^{\alpha}\Gamma(\alpha)}$$
	- For $x > 0$
	- The denominator is the normalizing constant.
	- We usually aren't interested in finding the area under the curve, but we may later come back to compute tail probabilities.
- Remark: By recognizing this pdf in one form another and using the fact
- $$\int\limits_0^{\infty} x^{\alpha - 1} e^{-\frac{x}{\beta}} dx = \beta^{\alpha} \Gamma(\alpha)$$
- Will allow us to compute $\mathbb{E}(X^n)$ $\forall$ $n$.
-
\begin{align*}
	\mathbb{E}(X) &= \int\limits_0^{\infty} x \cdot \frac{x^{\alpha - 1}e^{-\frac{x}{\beta}}}{\beta^{\alpha}\Gamma(\alpha)} dx \\
	&= \frac{1}{\beta^{\alpha}\Gamma(\alpha)} \int\limits_0^{\infty} x^{\alpha}e^{-\frac{x}{\beta}} dx \\
	&= \frac{1}{\beta^{\alpha}\Gamma(\alpha)} \beta^{\alpha + 1}\Gamma(\alpha + 1) \\
	&\text{This substitution is the "Normalization trick" - you don't always have to integrate it out} \\
	&= \frac{\beta^{\alpha + 1}\Gamma(\alpha + 1)}{\beta^{\alpha}\Gamma(\alpha)} \\
	&= \frac{\beta^{\alpha + 1} \alpha \Gamma(\alpha)}{\beta^{\alpha}\Gamma(\alpha)} \\
	&= \alpha \beta
\end{align*}
- Exercise: Show $\mathbb{E}(X^2) = \alpha(\alpha + 1)\beta^2$ by using the normalization trick

# Beta-family of pdf's
- Important for ordered statistics, Bayesian statistics
- We say $X \sim$ Beta($\alpha, \beta$) if $X$ has the pdf with $\alpha > 0, \beta > 0$
- $$f(x) = \frac{x^{\alpha - 1}(1 - x)^{\beta - 1}}{\int\limits_0^1 x^{\alpha - 1} (1 - x)^{\beta - 1} dx} $$
	- for $0 < x < 1$.
- Where, in fact, $\int\limits_0^1 x^{\alpha - 1} (1 - x)^{\beta - 1} dx = \frac{\Gamma(\alpha) \Gamma(\beta)}{\Gamma(\alpha + \beta)}$ (show this for extra credit)
- Therefore the pdf is 
- $$f(x) = \frac{\Gamma(\alpha + \beta)}{\Gamma(\alpha) \Gamma(\beta)} x^{\alpha - 1}(1 - x)^{\beta - 1}$$
	- for $0 < x < 1$.
- Exercise: Show $\mathbb{E}(x) = \frac{\alpha}{\alpha + \beta}$

# CDF technique
- Suppose $X \sim f_X(x)$
	- "$X$ is a random variable that has $f_X(x)$ as its pdf"
- And $Y = g(X)$. What is the pdf of Y?
- Example 1: Suppose $Z \sim$ Normal(0, 1)
	- $$\phi = \frac{e^-\frac{x^2}{2}}{\sqrt{2\pi}} \text{ for } -\infty < x < \infty$$
	- Find the pdf of $Y = Z^2$
	- Step 1: Compute the cdf of $Y$ in terms of the cdf of $X$
	- Step 2: Take a derivative and use use the chain rule
	- Step 1
		- Assume $y \geq 0$
		-
		\begin{align*}
			F_Y(y) &= P(Y \leq y) \\
			&= P(Z^2 \leq y) \\
			&= P(\lvert Z \rvert \leq \sqrt{y}) \\
			&= P(-\sqrt{y} \leq Z \leq \sqrt{y}) \\
			&= P(-\sqrt{y} < Z \leq \sqrt{y}) \\
			&= \Phi(\sqrt{y}) - \Phi(-\sqrt{y})
		\end{align*}
	- Step 2
		-
		\begin{align*}
			\frac{d}{dy}F_Y(y) &= f_Y(y) \\
			&= \frac{d}{dy}(\Phi(\sqrt{y}) - \Phi(-\sqrt{y})) \\
			&= \phi(\sqrt{y}) \frac{d}{dy}(\sqrt{y}) - \phi(-\sqrt{y}) \frac{d}{dy}(-\sqrt{y}) \\
			&= \phi(\sqrt{y}) \frac{d}{dy}(\sqrt{y}) + \phi(\sqrt{y}) \frac{d}{dy}(\sqrt{y}) \\
			&= \dots \\
			&= 2 \cdot \phi(\sqrt{y})\frac{1}{2\sqrt{y}} \\
			&= \frac{1}{\sqrt{y}} \phi(\sqrt{y}) \\
			&= \frac{1}{y^{\frac{1}{2}}} \cdot \frac{e^{-\frac{y}{2}}}{\sqrt{2\pi}} \\
			&= \frac{y^{-\frac{1}{2}} e^{-\frac{y}{2}}}{\sqrt{2\pi}} \text{ for } y > 0 \\
			&= \text{Gamma}(\frac{1}{2}, 2) \sim \chi_1^2
		\end{align*}
- Example 2: Suppose $Y = g(X)$ and $g$ is strictly monotone
	- Claim
	- $$f_Y(y) = f_X(g^{-1}(y)) \Big\lvert \frac{d}{dy} g^{-1}(y) \Big\rvert $$
	- Case 1: $g$ strictly increasing
		- 
		\begin{align*}
			F_Y(y) &= P(g(X) \leq y) \\
			&= P(X \leq g^{-1}(y)) \\
			&= F_X(g^{-1}(y))
		\end{align*}
		- $f_Y(y) = f_X(g^{-1}(y)) \cdot \frac{d}{dy}(g^{-1}(y))$
	- Case 2: $G$ decreasing
		- 
		\begin{align*}
			F_Y(y) &= P(g(X) \leq y) \\
			&= P(X \leq g^{-1}(y)) \\
			&= F_X(g^{-1}(y)) \\
			&= 1 - F_X(g^{-1}(y))
		\end{align*}
		- $f_Y(y) = -f_X(g^{-1}(y)) \cdot \frac{d}{dy}(-g^{-1}(y)) = f_X(g^{-1}(y)) \cdot \Big\lvert \frac{d}{dy}(-g^{-1}(y)) \Big\rvert$

# Weibull distribution
- $X \sim$ exp(1) $f_X(x) = e^{-x}$ for $x > 0$
- Find pdf of $Y = \nu + \alpha X^{\frac{1}{\beta}}$ ($\nu \in \mathbb{R}, \alpha > 0, \beta > 0$)