---
title: Intro Prob Lecture Notes
author:
    - William Sun
date:
    - March 17, 2017
geometry: margin=3cm
header-includes:
    - \usepackage{setspace}
    - \doublespacing
---
# The Normal($\mu, \sigma^2$) pdf
- $$f(x) = \frac{e^{-\frac{1}{2}(\frac{x - \mu}{\sigma})^2}}{\sigma \sqrt{2 \pi}} for - \infty < x < \infty$$
- When $\mu = 0$ and $\sigma = 1$ we call this the *standard normal pdf* and use the letter $\phi$ (Lowercase Greek 'phi')
	- Notation: In this class, $\mathbb{Z} \sim$ Normal(0, 1) *ALWAYS*
- $$\phi(x) = \frac{e^{-\frac{x^2}{2}}}{\sqrt{2\pi}} for -\infty < x < \infty$$
- The corresponding cdf is given the symbol $\Phi$ (Uppercase Greek 'Phi')
- $$\Phi(x) = \int\limits_{-\infty}^{\infty} \phi(u)du$$
	- This cdf is tabulated for values of x between 0.00 and 3.49 in increments of .01 on page 190 of the textbook
	- Check:
		- $P(\mathbb{Z} \leq 2.17) = \Phi(2.17) = .9850$
		- $P(\mathbb{Z} \leq 1.00) = \Phi(1.00) = .8413$
		- $P(\mathbb{Z} \leq 0.00) = \Phi(0.00) = .5$
	- Since this is a normal distribution, $P(\mathbb{Z} \leq -2.17) = 1 - P(\mathbb{Z} \leq 2.17)$
	- And in general, $\Phi(x) = 1 - \Phi(-x)$
- Last time: If $X \sim$ Normal($\mu, \sigma^2$), any $aX + b \sim$ Normal($a\mu + b, a^2\sigma^2$)
	- Example: $\mathbb{Z} \sim$ Normal(0, 1), $X = \sigma \mathbb{Z} + \mu \sim$ Normal($\mu, \sigma^2$)
	- Therefore, every random variable with a normal distribution is a linear transformation of a standard normal distribution and vice versa.
	$$ \implies \mathbb{Z} = \frac{X - \mu}{\sigma} \sim \text{Normal(0, 1)}$$
		- Z-score transformation (standardizing)
- Exercise: Show that both
	- $$\mathbb{E}(\mathbb{Z}) = \int\limits_{-\infty}^{\infty} z \cdot \frac{e^{- \frac{z^2}{2}}}{\sqrt{2 \pi}} dz = 0$$
	- $$\mathbb{E}(\mathbb{Z}^2) = \int\limits_{-\infty}^{\infty} z \cdot \frac{e^{- \frac{z^2}{2}}}{\sqrt{2 \pi}} dz = 1$$

# The Euler Gamma Function
- $$\Gamma(\alpha) = \int\limits_0^{\infty} y^{\alpha - 1}e^{-y} dy$$
	- Not defined at 0, negative even integers. However, it is defined for everywhere else in the complex plane. 
	- When $\alpha > 0$, it is defined in finite.
	- Note: Wikipedia has a beautiful drawing of this function
	- Generalizes the factorial
		- $$\Gamma(1) = \int\limits_0^{\infty} y^{0} e^{-y} dy = 1$$
		- Suppose $\alpha > 1$
	- 
	\begin{align*}
	\Gamma(\alpha) &= y^{\alpha - 1}e^{-y} dy\\
	& \text{Let } u = y^{\alpha - 1}, dv = e^{-y} dy \\
	&= y^{\alpha - 1}(-e^{-y}) \Big|_0^{\infty} - \int\limits_0^{\infty} - e^{-y} \cdot (\alpha - 1) y^{\alpha - 2} dy \\
	&= (\alpha - 1) \int\limits_0^{\infty} y^{\alpha - 2}e^{-y} dy \\
	&= (\alpha - 1) \Gamma(\alpha - 1)
	\end{align*}
		- This is known as the reduction property of $\Gamma(\alpha)$.
		- Ex: suppose $\alpha = 4$
			- $\Gamma(4) = 3 * \Gamma(3) = 3 * 2 * \Gamma(2) = 3 * 2 * 1 * \Gamma(1) = 3!$
		- Therefore, when $n > 0, n$ is integer, $\Gamma(n) = (n - 1)!$
		- Tricky fact: $\Gamma(\frac{1}{2}) = \sqrt{\pi}$ (see notes)
		- $\Gamma(\frac{7}{2}) = \frac{5 \cdot 3 \cdot 1}{2 \cdot 2 \cdot 2} \Gamma(\frac{1}{2}) = \frac{15\sqrt{\pi}}{8}$
		- $\Gamma(7.3) = (6.3)(5.3)(4.3)(3.3)(2.3)(1.3)(.3)\Gamma(.3)$
	- Suppose $\alpha > 0$ and $\beta > 0$. Integrate
	-
	\begin{align*}
	\int\limits_0^{\infty} x^{\alpha - 1}e^{-\frac{x}{\beta}} dx &=  \\
	& \text{Let } u = \frac{x}{\beta} \rightarrow x = \beta u, dx = \beta du \\
	&= \int\limits_0^{\infty} (\beta u)^{\alpha - 1} e^{-u} \beta du \\
	&= \beta^{\alpha} \Gamma(\alpha)
	\end{align*}
	- $$\int\limits_0^{\infty} x^{\alpha - 1}e^{-\frac{x}{\beta}} dx = \beta^{\alpha} \Gamma(\alpha)$$
	- Be smart:
	- $$\int\limits_0^{\infty} x^3 e^{-\frac{x}{2}} dx = w^4 \Gamma(4) = 16(6) = 96$$
	- $$\int\limits_0^{\infty} x^2 e^{-2x} = \frac{1}{2}^3 \Gamma(3) = \frac{1}{4}$$
	- We define 
	- $$f(x) = \frac{x^{\alpha - 1} e^{- \frac{x}{\beta}}}{\beta^{\alpha} \Gamma(\alpha)} \text{for } x > 0$$
	- As the Gamma($\alpha, \beta$) pdf
		- $\alpha$ is the shape parameter
		- $\beta$ is the scale parameter
	- Plug in $\alpha = 1$ in the Gamma($\alpha, \beta$) pdf
	- $$f(x) = \frac{e^{-\frac{x}{\beta}}}{\beta} = \frac{1}{\beta} e^{-\frac{x}{\beta}} \text{for } x > 0$$
	- Suppose $n > 1$ integer takes $\alpha = \frac{n}{2}$ and $\beta = 2$
	- $$f(x) = \frac{x^{\frac{n}{2} - 1} e^{-\frac{x}{2}}}{2^{\frac{n}{2}}\Gamma(\frac{n}{2})} \sim \chi^2_n$$
		- Chi-square with $n$ degrees of freedom (used in statistics)